Separate pre-interp, start alpha, prove single equiv, look at strict positivity
Separate pre-interp into domain and function/predicate, makes dependent
types nicer
With this, proved equivalence for inductive preds
Start some things about alpha conversion
Investigate strict positivity, give example to show why we need and why
lemma we wanted to prove is not true without it

proofs/core/Denotational.v
@@ -19,15 +19,15 @@ Definition all_dec : forall (P : Prop), {P} + {~P} := excluded_middle_informativ
 Section Denot.
 
 Context {sigma: sig} {gamma: context} (gamma_valid: valid_context sigma gamma)
-  (i: pre_interp gamma_valid).
+  (pd: pi_dom) (pf: pi_funpred gamma_valid pd).
 
 (*Representation of terms, formulas, patterns*)
 
-Notation domain := (domain (dom_aux gamma_valid i)).
-Notation val x :=  (v_subst (v_typevar gamma_valid i x)).
-Notation v_typevar := (v_typevar gamma_valid i).
-Notation funs := (funs gamma_valid i).
-Notation substi := (substi gamma_valid i).
+Notation domain := (domain (dom_aux pd)).
+Notation val x :=  (v_subst (v_typevar x)).
+Notation val_typevar := (@val_typevar sigma).
+Notation funs := (funs gamma_valid pd pf).
+Notation substi := (substi pd).
 
 (*TODO: 2 options: can take in hypothesis that term has type ty and then use
   dependent type obligations
@@ -36,8 +36,8 @@ Notation substi := (substi gamma_valid i).
   for now, use typing hypothesis - this makes the function stuff a bit easier
   and we shouldn't have to match on types everywhere
   *)
-
-Definition cast_dom_vty {v: val_typevar gamma_valid i} 
+(*TODO: HERE*)
+Definition cast_dom_vty {v: val_typevar} 
 {v1 v2: vty} (Heq: v1 = v2) (x: domain (val v v1)) : domain (val v v2).
 Proof.
   subst. apply x.
@@ -105,9 +105,9 @@ Proof.
   apply sort_inj. unfold v_subst; simpl.
   induction ty; simpl; auto.
   - destruct (in_dec typevar_eq_dec v0 params).
-     + assert (Hin:=i0). 
-       apply (ty_subst_fun_in params args vty_int v0 H) in i0; auto.
-       destruct i0 as [ty [Hinty Hty]]. rewrite !Hty.
+     + assert (Hin:=i). 
+       apply (ty_subst_fun_in params args vty_int v0 H) in i; auto.
+       destruct i as [ty [Hinty Hty]]. rewrite !Hty.
        apply (ty_subst_fun_in params (sorts_to_tys
        (map
           (fun t : vty =>
@@ -157,7 +157,7 @@ Proof.
 Qed.
 
 (*We use the above to get the arg list (tentatively)*)
-Definition get_arg_list (v: val_typevar gamma_valid i)
+Definition get_arg_list (v: val_typevar)
   (f: funsym) (vs: list vty) (ts: list term) 
   (reps: forall (t: term) (ty: vty),
     term_has_type sigma t ty ->
@@ -197,7 +197,7 @@ Qed.
 
 (*This is irrelevant in the choice of proof*)
 
-Lemma get_arg_list_irrel (v: val_typevar gamma_valid i)
+Lemma get_arg_list_irrel (v: val_typevar)
 (f: funsym) (vs: list vty) (ts: list term) 
 (reps: forall (t: term) (ty: vty),
   term_has_type sigma t ty ->
@@ -236,7 +236,7 @@ Proof.
 Qed.
  
 (*Also need a version for preds (TODO: can we reduce duplication?)*)
-Definition get_arg_list_pred (v: val_typevar gamma_valid i)
+Definition get_arg_list_pred (v: val_typevar)
   (p: predsym) (vs: list vty) (ts: list term) 
   (reps: forall (t: term) (ty: vty),
     term_has_type sigma t ty ->
@@ -263,7 +263,7 @@ Proof.
       * apply IHts; auto.
 Defined.
 
-Lemma get_arg_list_pred_irrel (v: val_typevar gamma_valid i)
+Lemma get_arg_list_pred_irrel (v: val_typevar)
 (p: predsym) (vs: list vty) (ts: list term) 
 (reps: forall (t: term) (ty: vty),
   term_has_type sigma t ty ->
@@ -638,7 +638,7 @@ Proof.
   - exact None.
   - destruct (find_ts_in_ctx t);[|exact None].
     exact (Some (fst p, snd p, t, 
-      proj1_sig (is_sort_cons_sorts t l (is_sort_cons t l i0)))).
+      proj1_sig (is_sort_cons_sorts t l (is_sort_cons t l i)))).
 Defined.
 
 (*TODO: do we need other direction?*)
@@ -654,7 +654,7 @@ Proof.
     apply find_ts_in_ctx_iff in Hf. destruct Hf as [Hmg [Ham Hat]]; 
     repeat split; auto; subst.
     apply sort_inj. simpl. f_equal. clear H. 
-    generalize dependent (is_sort_cons (adt_name a) l i0).
+    generalize dependent (is_sort_cons (adt_name a) l i).
     intros H.
     destruct (is_sort_cons_sorts (adt_name a) l H). simpl.
     rewrite <- e; reflexivity.
@@ -663,7 +663,7 @@ Qed.
 
 (*Want to prove: suppose that type is valid and we have valuation, 
   then val v ty is valid*)
-Lemma val_valid: forall (v: val_typevar gamma_valid i) (ty: vty),
+Lemma val_valid: forall (v: val_typevar) (ty: vty),
   valid_type sigma ty ->
   valid_type sigma (val v ty).
 Proof.
@@ -674,7 +674,7 @@ Proof.
 Qed. 
 
 (*We need info about lengths and validity of the srts list*)
-Lemma adt_srts_valid: forall {v ty m a ts srts},
+Lemma adt_srts_valid: forall {v: val_typevar}  {ty m a ts srts},
   is_sort_adt (val v ty) = Some (m, a, ts, srts) ->
   valid_type sigma ty ->
   valid_type sigma (typesym_to_sort (adt_name a) srts).
@@ -687,7 +687,7 @@ Proof.
 Qed.
 
 (*We need to know something about the lengths*)
-Lemma adt_srts_length_eq: forall {v ty m a ts srts},
+Lemma adt_srts_length_eq: forall {v: val_typevar} {ty m a ts srts},
   is_sort_adt (val v ty) = Some (m, a, ts, srts) ->
   valid_type sigma ty ->
   length srts = length (m_params m).
@@ -707,14 +707,14 @@ Variable all_unif: forall m,
   mut_in_ctx m gamma ->
   uniform m.
 
-Lemma val_sort_eq: forall v (s: sort),
+Lemma val_sort_eq: forall (v: val_typevar) (s: sort),
   s = val v s.
 Proof.
   intros. apply subst_sort_eq.
 Qed.
 
 (*Need to know that all sorts are valid types*)
-Lemma adts_srts_valid: forall {v ty m a ts srts c},
+Lemma adts_srts_valid: forall {v : val_typevar} {ty m a ts srts c},
   is_sort_adt (val v ty) = Some (m, a, ts, srts) ->
   valid_type sigma ty ->
   constr_in_adt c a ->
@@ -758,7 +758,7 @@ Qed.
   [find_constr_rep] and casting.
   *)
 
-Fixpoint match_val_single (v: val_typevar gamma_valid i) (ty: vty)
+Fixpoint match_val_single (v: val_typevar) (ty: vty)
   (Hval: valid_type sigma ty)
   (d: domain (val v ty))
   (p: pattern) {struct p} : 
@@ -796,8 +796,8 @@ Fixpoint match_val_single (v: val_typevar gamma_valid i) (ty: vty)
       | conj Hseq (conj a_in (conj m_in Htseq)) =>
         (*We cast to get an ADT, now that we know that this actually is
           an ADT*)
-        let adt : adt_rep m srts (dom_aux gamma_valid i) a a_in :=
-          scast (adts gamma_valid i m srts a a_in) (dom_cast _ Hseq d) in
+        let adt : adt_rep m srts (dom_aux pd) a a_in :=
+          scast (adts pd m srts a a_in) (dom_cast _ Hseq d) in
        
         (*Need a lemma about lengths for [find_constr_rep]*)
         let lengths_eq : length srts = length (m_params m) := 
@@ -806,7 +806,7 @@ Fixpoint match_val_single (v: val_typevar gamma_valid i) (ty: vty)
         (*The key part: get the constructor c and arg_list a
           such that d = [[c(a)]]*)
         let Hrep := find_constr_rep gamma_valid m m_in srts lengths_eq 
-          (dom_aux gamma_valid i) a a_in (adts gamma_valid i m srts) 
+          (dom_aux pd) a a_in (adts pd m srts) 
           (all_unif m m_in) adt in
 
         (*The different parts of Hrep we need*)
@@ -862,7 +862,7 @@ Fixpoint match_val_single (v: val_typevar gamma_valid i) (ty: vty)
     end eq_refl
   end.
 
-Lemma match_val_single_typs (v: val_typevar gamma_valid i) (ty: vty)
+Lemma match_val_single_typs (v: val_typevar) (ty: vty)
 (Hval: valid_type sigma ty)
 (d: domain (val v ty))
 (p: pattern) l:
@@ -893,18 +893,18 @@ Proof.
     destruct (funsym_eq_dec
     (projT1
       (find_constr_rep gamma_valid m Hincts srts
-          (Hsrtslen m adt ts srts eq_refl Hval) (dom_aux gamma_valid i) adt
-          Hinmut (adts gamma_valid i m srts) (all_unif m Hincts)
-          (scast (adts gamma_valid i m srts adt Hinmut)
-            (dom_cast (dom_aux gamma_valid i) Hvaleq d)))) f); 
+          (Hsrtslen m adt ts srts eq_refl Hval) (dom_aux pd) adt
+          Hinmut (adts pd m srts) (all_unif m Hincts)
+          (scast (adts pd m srts adt Hinmut)
+            (dom_cast (dom_aux pd) Hvaleq d)))) f); 
             [|intros ? C; inversion C].
     (*Need nested induction: simplify first*)
     generalize dependent (find_constr_rep gamma_valid m Hincts srts
     (Hsrtslen m adt ts srts eq_refl Hval) 
-    (dom_aux gamma_valid i) adt Hinmut (adts gamma_valid i m srts)
+    (dom_aux pd) adt Hinmut (adts pd m srts)
     (all_unif m Hincts)
-    (scast (adts gamma_valid i m srts adt Hinmut)
-      (dom_cast (dom_aux gamma_valid i) Hvaleq d))).
+    (scast (adts pd m srts adt Hinmut)
+      (dom_cast (dom_aux pd) Hvaleq d))).
     intros constr. destruct constr as [f' Hf']. simpl. intros Hf; subst.
     generalize dependent ((Hsrtsvalid m adt (adt_name adt) srts f eq_refl Hval (fst (proj1_sig Hf')))).
     destruct Hf'. simpl. clear e.
@@ -956,7 +956,7 @@ Lemma find_constr_rep_irrel (m: mut_adt) (m_in mut_in_ctx m gamma)
   (srts: list sort)
 *)
 (*TODO: move below prob*)
-Lemma match_val_single_irrel (v: val_typevar gamma_valid i) (ty: vty)
+Lemma match_val_single_irrel (v: val_typevar) (ty: vty)
 (Hval1 Hval2: valid_type sigma ty)
 (d: domain (val v ty))
 (p: pattern) :
@@ -985,17 +985,17 @@ Proof.
     destruct (funsym_eq_dec
     (projT1
        (find_constr_rep gamma_valid m Hincts srts
-          (Hsrtslen m adt ts srts eq_refl Hval2) (dom_aux gamma_valid i) adt
-          Hinmut (adts gamma_valid i m srts) (all_unif m Hincts)
-          (scast (adts gamma_valid i m srts adt Hinmut)
-             (dom_cast (dom_aux gamma_valid i) Hvaleq d)))) f); auto.
+          (Hsrtslen m adt ts srts eq_refl Hval2) (dom_aux pd) adt
+          Hinmut (adts pd m srts) (all_unif m Hincts)
+          (scast (adts pd m srts adt Hinmut)
+             (dom_cast (dom_aux pd) Hvaleq d)))) f); auto.
     (*Need nested induction: simplify first*)
     generalize dependent (find_constr_rep gamma_valid m Hincts srts
     (Hsrtslen m adt ts srts eq_refl Hval2) 
-    (dom_aux gamma_valid i) adt Hinmut (adts gamma_valid i m srts)
+    (dom_aux pd) adt Hinmut (adts pd m srts)
     (all_unif m Hincts)
-    (scast (adts gamma_valid i m srts adt Hinmut)
-       (dom_cast (dom_aux gamma_valid i) Hvaleq d))).
+    (scast (adts pd m srts adt Hinmut)
+       (dom_cast (dom_aux pd) Hvaleq d))).
     intros constr. destruct constr as [f' Hf']. simpl. intros Hf; subst.
     generalize dependent ((Hsrtsvalid m adt (adt_name adt) srts f eq_refl Hval1 (fst (proj1_sig Hf')))).
     generalize dependent ((Hsrtsvalid m adt (adt_name adt) srts f eq_refl Hval2 (fst (proj1_sig Hf')))).
@@ -1007,7 +1007,7 @@ Proof.
     + destruct ps; auto.
     + inversion H; subst. reflexivity.
       (*Don't know why we need to expand map*)
-      rewrite (H0 a (dom_cast (dom_aux gamma_valid i) (val_sort_eq v a) (hlist_hd a0))
+      rewrite (H0 a (dom_cast (dom_aux pd) (val_sort_eq v a) (hlist_hd a0))
         _ ((@Forall_inv vty (valid_type sigma) (sort_to_ty a)
       ((fix map (s : list sort) : list vty :=
           match s return (list vty) with
@@ -1021,7 +1021,7 @@ Proof.
           | nil => @nil vty
           | cons x0 s' => @cons vty (sort_to_ty x0) (map s')
           end) l) f0)
-      (dom_cast (dom_aux gamma_valid i) (val_sort_eq v a) (hlist_hd a0)) x) eqn : Hm; auto.
+      (dom_cast (dom_aux pd) (val_sort_eq v a) (hlist_hd a0)) x) eqn : Hm; auto.
       match goal with 
       | |- match ?o1 with | Some x => ?a | None => ?b end =
         match ?o2 with | Some y => ?c | None => ?d end =>
@@ -1040,10 +1040,10 @@ Definition get_assoc_list {A B: Set} (eq_dec: forall (x y: A), {x = y} + { x <> 
 (*Look up each entry in the list, if the name or type doesn't
   match, default to existing val*)
 (*Usefully, Coq can tell that this does not affect v_typevar*)
-Definition extend_val_with_list (v: val_typevar gamma_valid i) 
-  (vv: val_vars gamma_valid i v)
+Definition extend_val_with_list (v: val_typevar) 
+  (vv: val_vars pd v)
   (l: list (vsymbol * {t: vty & domain (val v t) })) :
-  val_vars gamma_valid i v.
+  val_vars pd v.
 intros x.
   destruct (get_assoc_list vsymbol_eq_dec l x).
   + destruct (vty_eq_dec (snd x) (projT1 s)).
@@ -1106,7 +1106,7 @@ Proof.
 Qed.*)
 
 (*TODO: move above?*)
-Variable vt: val_typevar gamma_valid i.
+Variable vt: val_typevar.
 
 (*Inversion lemma for patterns*)
 
@@ -1120,7 +1120,7 @@ Variable vt: val_typevar gamma_valid i.
   the types work out. In each case, we separate the hypotheses and give
   explicit types for clarity. The final result is often quite simple and just
   needs 1 or more casts for dependent type purposes. *)
-Fixpoint term_rep (v: val_vars gamma_valid i vt) (t: term) (ty: vty)
+Fixpoint term_rep (v: val_vars pd vt) (t: term) (ty: vty)
   (Hty: term_has_type sigma t ty) {struct t} : domain (val vt ty) :=
   (match t as tm return t = tm -> domain (val vt ty) with
   | Tconst (ConstInt z) => fun Htm =>
@@ -1139,7 +1139,7 @@ Fixpoint term_rep (v: val_vars gamma_valid i vt) (t: term) (ty: vty)
     cast_dom_vty Htyeq r (*(r_to_dom _ _ _ _ v r)*)
   | Tvar x => fun Htm =>
     let Heq : ty = snd x := ty_var_inv (has_type_eq Htm Hty) in
-    (dom_cast _ (f_equal (val vt) (eq_sym Heq)) (var_to_dom _ _ vt v x))
+    (dom_cast _ (f_equal (val vt) (eq_sym Heq)) (var_to_dom _ vt v x))
     (*dom_cast _ (f_equal (v_vars _ v) Heq)*) 
     (*ltac:(rewrite Heq; exact (var_to_dom _ _ v x))*)
 
@@ -1162,7 +1162,7 @@ Fixpoint term_rep (v: val_vars gamma_valid i vt) (t: term) (ty: vty)
       types work out*)
   
     cast_dom_vty Htyeq (
-      dom_cast (dom_aux gamma_valid i)
+      dom_cast (dom_aux pd)
         (eq_sym Heqret)
           ((funs f (map (val vt) vs)) 
             (get_arg_list vt f vs ts (term_rep v) (ex_intro _ ty Hty'))))
@@ -1216,7 +1216,7 @@ Fixpoint term_rep (v: val_vars gamma_valid i vt) (t: term) (ty: vty)
         | None => match_rep ptl (Forall_inv_tail Hall)
         end
       | _ => (*TODO: show we cannot reach this*) fun _ =>
-        match domain_ne gamma_valid i (val vt ty) with
+        match domain_ne pd (val vt ty) with
         | DE x =>  x
         end
       end Hall in
@@ -1228,7 +1228,7 @@ Fixpoint term_rep (v: val_vars gamma_valid i vt) (t: term) (ty: vty)
       let Heq : ty = snd x := proj2 (ty_eps_inv Hty') in
       (*We need to show that domain (val v ty) is inhabited*)
       let def : domain (val vt ty) :=
-      match (domain_ne gamma_valid i (val vt ty)) with
+      match (domain_ne pd (val vt ty)) with
       | DE x => x 
       end in
       (*Semantics for epsilon - use Coq's classical epsilon,
@@ -1242,7 +1242,7 @@ Fixpoint term_rep (v: val_vars gamma_valid i vt) (t: term) (ty: vty)
 
   end) eq_refl
 
-with formula_rep (v: val_vars gamma_valid i vt) (f: formula) 
+with formula_rep (v: val_vars pd vt) (f: formula) 
   (Hval: valid_formula sigma f) {struct f} : bool :=
   (match f as fmla return f = fmla -> bool with
   | Ftrue => fun _ => true
@@ -1289,7 +1289,7 @@ with formula_rep (v: val_vars gamma_valid i vt) (f: formula)
     let Hval': valid_formula sigma (Fpred p vs ts) :=
       valid_formula_eq Hf Hval in
 
-    preds _ _ p (map (val vt) vs)
+    preds _ _ pf p (map (val vt) vs)
       (get_arg_list_pred vt p vs ts (term_rep v) Hval')
 
   | Fquant Tforall x f' => fun Hf =>
@@ -1363,10 +1363,10 @@ with formula_rep (v: val_vars gamma_valid i vt) (f: formula)
 
 Require Import FunctionalExtensionality.
 Lemma term_form_rep_irrel: forall (tm: term) (f: formula),
-  (forall (v: val_vars gamma_valid i vt) (ty: vty) (Hty1 Hty2:
+  (forall (v: val_vars pd vt) (ty: vty) (Hty1 Hty2:
     term_has_type sigma tm ty), 
       term_rep v tm ty Hty1 = term_rep v tm ty Hty2) /\
-  (forall (v: val_vars gamma_valid i vt) (Hval1 Hval2:
+  (forall (v: val_vars pd vt) (Hval1 Hval2:
     valid_formula sigma f), 
       formula_rep v f Hval1 = formula_rep v f Hval2).
 Proof.
@@ -1412,7 +1412,7 @@ Proof.
   - (*TODO: is this possible without funext?*)
     f_equal. apply functional_extensionality_dep.
     intros x.
-    rewrite (H (substi vt v0 v (dom_cast (dom_aux gamma_valid i)
+    rewrite (H (substi vt v0 v (dom_cast (dom_aux pd)
     (f_equal (val vt) (proj2 (ty_eps_inv (has_type_eq eq_refl Hty1)))) x))
       (proj1 (ty_eps_inv (has_type_eq eq_refl Hty1)))
     (proj1 (ty_eps_inv (has_type_eq eq_refl Hty2)))).
@@ -1428,9 +1428,9 @@ Proof.
       destruct (all_dec P); simpl; auto end.
     + exfalso. apply n. intros d.
       erewrite (H (substi vt v0 v d)).
-      apply i0.
+      apply i.
     + exfalso. apply n. intros d.
-      erewrite H. apply i0.
+      erewrite H. apply i.
     + exfalso. apply n. 
       destruct e as [d Hd].
       exists d. erewrite H. apply Hd.
@@ -1464,14 +1464,14 @@ Proof.
       apply IHps. auto.
 Qed.
 
-Lemma term_rep_irrel (v: val_vars gamma_valid i vt) (tm: term)
+Lemma term_rep_irrel (v: val_vars pd vt) (tm: term)
   (ty: vty) (Hty1 Hty2: term_has_type sigma tm ty) :
   term_rep v tm ty Hty1 = term_rep v tm ty Hty2.
 Proof.
   apply term_form_rep_irrel. apply Ftrue.
 Qed.
 
-Lemma fmla_rep_irrel (v: val_vars gamma_valid i vt) (f: formula)
+Lemma fmla_rep_irrel (v: val_vars pd vt) (f: formula)
     (Hval1 Hval2: valid_formula sigma f) :
   formula_rep v f Hval1 = formula_rep v f Hval2.
 Proof.
@@ -1488,14 +1488,34 @@ Section Alpha.
 (*Substitute y for all free ocurrences of x*)
 
 (*TODO: remove this: same as pat_fv*)
-Fixpoint pattern_boundvars (p: pattern) : list vsymbol :=
+Fixpoint bnd_p (p: pattern) : list vsymbol :=
   match p with
   | Pvar v => [v]
-  | Pconstr f tys ps => concat (map pattern_boundvars ps)
+  | Pconstr f tys ps => concat (map bnd_p ps)
   | Pwild => nil
-  | Por p1 p2 => (pattern_boundvars p1) ++ (pattern_boundvars p2)
-  | Pbind p1 v => v :: (pattern_boundvars p1)
+  | Por p1 p2 => (bnd_p p1) ++ (bnd_p p2)
+  | Pbind p1 v => v :: (bnd_p p1)
   end.
+
+Lemma or_false_r (P: Prop):
+  (P \/ False) <-> P.
+Proof.
+  split; intros; auto. destruct H; auto. destruct H.
+Qed.
+
+Lemma bnd_fv_p (p: pattern):
+  forall x, In x (bnd_p p) <-> In x (pat_fv p).
+Proof.
+  intros x. induction p; simpl; try reflexivity.
+  - induction ps; simpl; try reflexivity.
+    inversion H; subst. specialize (IHps H3).
+    rewrite in_app_iff, H2, union_elts, IHps.
+    reflexivity.
+  - rewrite in_app_iff, union_elts, IHp1, IHp2.
+    reflexivity.
+  - rewrite union_elts, or_comm, IHp. simpl. 
+    rewrite or_false_r. reflexivity.
+Qed.
 
 Fixpoint sub_f (x y: vsymbol) (f: formula) : formula :=
   match f with
@@ -1518,7 +1538,7 @@ Fixpoint sub_f (x y: vsymbol) (f: formula) : formula :=
     Fif (sub_f x y f1) (sub_f x y f2) (sub_f x y f3)
   | Fmatch tm ty ps =>
     Fmatch (sub_t x y tm) ty
-      (map (fun p => if in_bool vsymbol_eq_dec x (pat_fv (fst p)) then
+      (map (fun p => if in_bool vsymbol_eq_dec x (bnd_p (fst p)) then
         p else (fst p, sub_f x y (snd p))) ps)
   end
 with sub_t (x y: vsymbol) (t: term) : term :=
@@ -1536,7 +1556,7 @@ with sub_t (x y: vsymbol) (t: term) : term :=
     Tif (sub_f x y f1) (sub_t x y t1) (sub_t x y t2)
   | Tmatch tm ty ps =>
     Tmatch (sub_t x y tm) ty
-    (map (fun p => if in_bool vsymbol_eq_dec x (pat_fv (fst p)) then
+    (map (fun p => if in_bool vsymbol_eq_dec x (bnd_p (fst p)) then
       p else (fst p, sub_t x y (snd p))) ps)
   | Teps f1 v =>
     (*TODO: is this correct?*)
@@ -1595,7 +1615,7 @@ Fixpoint bnd_f (f: formula) : list vsymbol :=
     bnd_f f1 ++ bnd_f f2 ++ bnd_f f3
   | Fmatch tm ty ps =>
     bnd_t tm ++ concat (map 
-      (fun p => pat_fv (fst p) ++ bnd_f (snd p)) ps)
+      (fun p => bnd_p (fst p) ++ bnd_f (snd p)) ps)
   end
 with bnd_t (t: term) : list vsymbol :=
   match t with
@@ -1610,7 +1630,7 @@ with bnd_t (t: term) : list vsymbol :=
     bnd_f f1 ++ bnd_t t1 ++ bnd_t t2
   | Tmatch tm ty ps =>
     bnd_t tm ++ concat (map
-      (fun p => pat_fv (fst p) ++ bnd_t (snd p)) ps)
+      (fun p => bnd_p (fst p) ++ bnd_t (snd p)) ps)
   | Teps f1 v =>
     v :: bnd_f f1
     (*TODO: is this correct?*)
@@ -1734,17 +1754,13 @@ Proof.
   split; intros; auto. destruct H; auto.
 Qed.
 
-Lemma or_false_r (P: Prop):
-  (P \/ False) <-> P.
-Proof.
-  split; intros; auto. destruct H; auto. destruct H.
-Qed.
+
 
 (*Lemma for [match_val_single]*)
 Lemma match_var_single_free_var ty Hval d p l x ty'
   (Hpat: pattern_has_type sigma p ty'):
   match_val_single vt ty Hval d p = Some l ->
-  In x (pat_fv p) <-> In x (map fst l).
+  In x (bnd_p p) <-> In x (map fst l).
 Proof.
   revert Hval d l. generalize dependent ty'. 
   generalize dependent ty.
@@ -1772,18 +1788,18 @@ Proof.
     destruct (funsym_eq_dec
     (projT1
        (find_constr_rep gamma_valid m Hincts srts
-          (Hsrtslen m adt ts srts eq_refl Hval) (dom_aux gamma_valid i) adt
-          Hinmut (adts gamma_valid i m srts) (all_unif m Hincts)
-          (scast (adts gamma_valid i m srts adt Hinmut)
-             (dom_cast (dom_aux gamma_valid i) Hvaleq d)))) f); 
+          (Hsrtslen m adt ts srts eq_refl Hval) (dom_aux pd) adt
+          Hinmut (adts pd m srts) (all_unif m Hincts)
+          (scast (adts pd m srts adt Hinmut)
+             (dom_cast (dom_aux pd) Hvaleq d)))) f); 
              [|intros ? C; inversion C].
     (*Need nested induction: simplify first*)
     generalize dependent (find_constr_rep gamma_valid m Hincts srts
     (Hsrtslen m adt ts srts eq_refl Hval) 
-    (dom_aux gamma_valid i) adt Hinmut (adts gamma_valid i m srts)
+    (dom_aux pd) adt Hinmut (adts pd m srts)
     (all_unif m Hincts)
-    (scast (adts gamma_valid i m srts adt Hinmut)
-       (dom_cast (dom_aux gamma_valid i) Hvaleq d))).
+    (scast (adts pd m srts adt Hinmut)
+       (dom_cast (dom_aux pd) Hvaleq d))).
     intros constr. destruct constr as [f' Hf']. simpl. intros Hf; subst.
     generalize dependent ((Hsrtsvalid m adt (adt_name adt) srts f eq_refl Hval (fst (proj1_sig Hf')))).
     destruct Hf'. simpl. clear e.
@@ -1812,27 +1828,26 @@ Proof.
       inversion H9; subst. simpl in H4.
       apply (H2 _(ty_subst (s_params f) vs v)) in Hmatch; auto.
       apply (IHl args) in Hmatch0; auto.
-      simpl. rewrite union_elts, map_app, in_app_iff, Hmatch, Hmatch0.
+      simpl. rewrite map_app, !in_app_iff, Hmatch, Hmatch0.
       reflexivity.
   - simpl. intros. inversion H; subst. reflexivity.
   - simpl. intros. destruct (match_val_single vt ty Hval d p1) eqn: Hm.
     + inversion H; subst. inversion Hpat; subst.
       apply (IHp1 _ ty') in Hm; auto.
-      rewrite union_elts, Hm. rewrite <- H6, Hm, or_idem.
+      rewrite in_app_iff, Hm, bnd_fv_p. 
+      rewrite <- H6, <- bnd_fv_p, Hm, or_idem. 
       reflexivity.
     + inversion Hpat; subst.
       apply (IHp2 _ ty') in H; auto.
-      rewrite union_elts, H. rewrite <- H, H6, or_idem. 
+      rewrite in_app_iff, H, bnd_fv_p. 
+      rewrite H6, <- bnd_fv_p, H, or_idem.
       reflexivity.
   - simpl. intros.
     destruct (match_val_single vt ty Hval d p) eqn : Hm.
-    + inversion H; subst. simpl.
-      rewrite union_elts. simpl.
+    + destruct (vty_eq_dec (snd v) ty); inversion H; subst. simpl.
       inversion Hpat; subst.
       apply (IHp _ (snd v)) in Hm; auto.
-      rewrite Hm, or_comm, or_false_r.
-      destruct (vty_eq_dec (snd v) ty); subst; inversion H; subst.
-      reflexivity. 
+      rewrite Hm. reflexivity.
     + inversion H.
 Qed.
 
@@ -1862,7 +1877,7 @@ Proof.
     apply IHl. intro C. apply H. right; assumption.
 Qed.
 
-Lemma extend_val_with_list_in (vv: val_vars gamma_valid i vt) 
+Lemma extend_val_with_list_in (vv: val_vars pd vt) 
   (x: vsymbol)
   (d: domain (val vt (snd x))) (l: list (vsymbol * {t : vty & domain (val vt t)}))
   (Hl: forall x y, In (x, y) l -> projT1 y = snd x):
@@ -1883,7 +1898,7 @@ Proof.
     subst. contradiction.
 Qed.
 
-Lemma extend_val_with_list_notin (vv: val_vars gamma_valid i vt) 
+Lemma extend_val_with_list_notin (vv: val_vars pd vt) 
   (x: vsymbol)
   (d: domain (val vt (snd x))) (l: list (vsymbol * {t : vty & domain (val vt t)}))
   (Hl: forall x y, In (x, y) l -> projT1 y = snd x):
@@ -1904,7 +1919,7 @@ Qed.
 (*TODO: see if we can get rid of casting in Here*)
 Lemma sub_correct (t: term) (f: formula) :
   (forall (x y: vsymbol) (Heq: snd x = snd y) 
-    (v: val_vars gamma_valid i vt) (ty: vty) 
+    (v: val_vars pd vt) (ty: vty) 
     (Hty1: term_has_type sigma t ty)
     (Hty2: term_has_type sigma (sub_t x y t) ty)
     (Hfree: ~In y (bnd_t t)),
@@ -1913,7 +1928,7 @@ Lemma sub_correct (t: term) (f: formula) :
       (v y))) t ty Hty1 =
     term_rep v (sub_t x y t) ty Hty2) /\
   (forall (x y: vsymbol) (Heq: snd x = snd y) 
-    (v: val_vars gamma_valid i vt)
+    (v: val_vars pd vt)
     (Hval1: valid_formula sigma f)
     (Hval2: valid_formula sigma (sub_f x y f))
     (Hfree: ~In y (bnd_f f)),
@@ -2052,11 +2067,11 @@ Proof.
     simpl in Hty2.
     generalize dependent (proj1 (ty_match_inv (@has_type_eq sigma
     (Tmatch (sub_t x y tm) v
-    (map (fun p => if in_bool vsymbol_eq_dec x (pat_fv (fst p)) then
+    (map (fun p => if in_bool vsymbol_eq_dec x (bnd_p (fst p)) then
       p else (fst p, sub_t x y (snd p))) ps)) _ _ eq_refl Hty2))).
     generalize dependent (proj2 (ty_match_inv (@has_type_eq sigma
     (Tmatch (sub_t x y tm) v
-    (map (fun p => if in_bool vsymbol_eq_dec x (pat_fv (fst p)) then
+    (map (fun p => if in_bool vsymbol_eq_dec x (bnd_p (fst p)) then
       p else (fst p, sub_t x y (snd p))) ps)) _ _ eq_refl Hty2))).
     clear Hty2. 
     intros Hall1 Hty1 Hall2 Hty2. (*for better names*)
@@ -2066,17 +2081,17 @@ Proof.
     destruct (match_val_single vt v (has_type_valid gamma_valid tm v Hty2)
     (term_rep
        (substi vt v0 x
-          (dom_cast (dom_aux gamma_valid i) (f_equal (val vt) (eq_sym Heq))
+          (dom_cast (dom_aux pd) (f_equal (val vt) (eq_sym Heq))
              (v0 y))) tm v Hty2) p1) as [newval |] eqn : Hmatch.
     + revert Hall1. simpl.
-      destruct (in_bool vsymbol_eq_dec x (pat_fv p1)) eqn : Hinp1.
+      destruct (in_bool vsymbol_eq_dec x (bnd_p p1)) eqn : Hinp1.
       * intros.
         rewrite <- H with(Heq:=Heq) (Hty1:=Hty2) by solve_bnd.
         rewrite match_val_single_irrel with (Hval2:=(has_type_valid gamma_valid tm v Hty2)).
         rewrite Hmatch.
         assert (In x (map fst newval)). {
           apply (match_var_single_free_var) with(x:=x)(ty':=v) in Hmatch.
-          apply Hmatch. destruct (in_bool_spec vsymbol_eq_dec x (pat_fv p1)); auto.
+          apply Hmatch. destruct (in_bool_spec vsymbol_eq_dec x (bnd_p p1)); auto.
           inversion Hinp1.
           specialize (Hallpats (p1, t1)). apply Hallpats. left; auto.
        }
@@ -2092,7 +2107,7 @@ Proof.
         assert (~In x (map fst newval)). {
           apply (match_var_single_free_var) with(x:=x)(ty':=v) in Hmatch.
           intro C.
-          apply Hmatch in C. destruct (in_bool_spec vsymbol_eq_dec x (pat_fv p1)); auto.
+          apply Hmatch in C. destruct (in_bool_spec vsymbol_eq_dec x (bnd_p p1)); auto.
           inversion Hinp1.
           specialize (Hallpats (p1, t1)). apply Hallpats. left; auto.
        }
@@ -2106,7 +2121,7 @@ Proof.
        apply get_assoc_list_some in Ha.
        apply match_var_single_free_var with(x:=y)(ty':=v) in Hmatch.
        exfalso. apply Hfree. simpl.
-       assert (In y (pat_fv p1)). apply Hmatch. rewrite in_map_iff.
+       assert (In y (bnd_p p1)). apply Hmatch. rewrite in_map_iff.
        exists (y, s). split; auto.
        solve_bnd.
        specialize (Hallpats (p1, t1)). apply Hallpats. left; auto.
@@ -2118,7 +2133,7 @@ Proof.
           (basically a bigger [substi_diff]), then we apply
           the IH (the Forall one)*)
     + revert Hall1. simpl.  
-      destruct (in_bool vsymbol_eq_dec x (pat_fv p1)) eqn : Hinp1.
+      destruct (in_bool vsymbol_eq_dec x (bnd_p p1)) eqn : Hinp1.
       * intros.
         rewrite <- H with(Heq:=Heq) (Hty1:=Hty2) by solve_bnd.
         rewrite match_val_single_irrel with (Hval2:=(has_type_valid gamma_valid tm v Hty2)).
@@ -2252,17 +2267,17 @@ Proof.
     destruct (match_val_single vt v (has_type_valid gamma_valid tm v Hty2)
     (term_rep
        (substi vt v0 x
-          (dom_cast (dom_aux gamma_valid i) (f_equal (val vt) (eq_sym Heq))
+          (dom_cast (dom_aux pd) (f_equal (val vt) (eq_sym Heq))
              (v0 y))) tm v Hty2) p1) as [newval |] eqn : Hmatch.
     + revert Hall1. simpl.
-      destruct (in_bool vsymbol_eq_dec x (pat_fv p1)) eqn : Hinp1.
+      destruct (in_bool vsymbol_eq_dec x (bnd_p p1)) eqn : Hinp1.
       * intros.
         rewrite <- H with(Heq:=Heq) (Hty1:=Hty2) by solve_bnd.
         rewrite match_val_single_irrel with (Hval2:=(has_type_valid gamma_valid tm v Hty2)).
         rewrite Hmatch.
         assert (In x (map fst newval)). {
           apply (match_var_single_free_var) with(x:=x)(ty':=v) in Hmatch.
-          apply Hmatch. destruct (in_bool_spec vsymbol_eq_dec x (pat_fv p1)); auto.
+          apply Hmatch. destruct (in_bool_spec vsymbol_eq_dec x (bnd_p p1)); auto.
           inversion Hinp1.
           inversion Hallpats; subst. exact H3.
        }
@@ -2278,7 +2293,7 @@ Proof.
         assert (~In x (map fst newval)). {
           apply (match_var_single_free_var) with(x:=x)(ty':=v) in Hmatch.
           intro C.
-          apply Hmatch in C. destruct (in_bool_spec vsymbol_eq_dec x (pat_fv p1)); auto.
+          apply Hmatch in C. destruct (in_bool_spec vsymbol_eq_dec x (bnd_p p1)); auto.
           inversion Hinp1.
           inversion Hallpats; subst. exact H4.
         }
@@ -2292,7 +2307,7 @@ Proof.
        apply get_assoc_list_some in Ha.
        apply match_var_single_free_var with(x:=y)(ty':=v) in Hmatch.
        exfalso. apply Hfree. simpl.
-       assert (In y (pat_fv p1)). apply Hmatch. rewrite in_map_iff.
+       assert (In y (bnd_p p1)). apply Hmatch. rewrite in_map_iff.
        exists (y, s). split; auto.
        solve_bnd.
        inversion Hallpats; subst. auto.
@@ -2304,7 +2319,7 @@ Proof.
           (basically a bigger [substi_diff]), then we apply
           the IH (the Forall one)*)
     + revert Hall1. simpl.  
-      destruct (in_bool vsymbol_eq_dec x (pat_fv p1)) eqn : Hinp1.
+      destruct (in_bool vsymbol_eq_dec x (bnd_p p1)) eqn : Hinp1.
       * intros.
         rewrite <- H with(Heq:=Heq) (Hty1:=Hty2) by solve_bnd.
         rewrite match_val_single_irrel with (Hval2:=(has_type_valid gamma_valid tm v Hty2)).
@@ -2341,7 +2356,7 @@ Qed.
 (*The useful versions:*)
 Corollary sub_t_correct (t: term) (x y: vsymbol)
   (Heq: snd x = snd y)
-  (v: val_vars gamma_valid i vt) (ty: vty)
+  (v: val_vars pd vt) (ty: vty)
   (Hty1: term_has_type sigma t ty)
   (Hty2: term_has_type sigma (sub_t x y t) ty)
   (Hfree: ~In y (bnd_t t)):
@@ -2355,7 +2370,7 @@ Qed.
 
 Corollary sub_f_correct (f: formula)
   (x y: vsymbol) (Heq: snd x = snd y) 
-  (v: val_vars gamma_valid i vt)
+  (v: val_vars pd vt)
   (Hval1: valid_formula sigma f)
   (Hval2: valid_formula sigma (sub_f x y f))
   (Hfree: ~In y (bnd_f f)):
@@ -2370,11 +2385,11 @@ Qed.
 (*Other lemma we need: a term/formula is interpreted the
   same on all valuations that agree on the free variables*)
 Lemma val_fv_agree (t: term) (f: formula) :
-(forall (v1 v2: val_vars gamma_valid i vt) (ty: vty) 
+(forall (v1 v2: val_vars pd vt) (ty: vty) 
   (Hty: term_has_type sigma t ty),
   (forall x, In x (term_fv t) -> v1 x = v2 x) ->
   term_rep v1 t ty Hty = term_rep v2 t ty Hty) /\
-(forall (v1 v2: val_vars gamma_valid i vt) 
+(forall (v1 v2: val_vars pd vt) 
   (Hval: valid_formula sigma f),
   (forall x, In x (form_fv f) -> v1 x = v2 x) ->
   formula_rep v1 f Hval = formula_rep v2 f Hval).
@@ -2438,7 +2453,7 @@ Admitted.
 
 (*Corollaries:*)
 Corollary term_fv_agree (t: term)
-  (v1 v2: val_vars gamma_valid i vt) (ty: vty) 
+  (v1 v2: val_vars pd vt) (ty: vty) 
   (Hty: term_has_type sigma t ty):
   (forall x, In x (term_fv t) -> v1 x = v2 x) ->
   term_rep v1 t ty Hty = term_rep v2 t ty Hty.
@@ -2447,7 +2462,7 @@ Proof.
 Qed.
 
 Corollary form_fv_agree (f: formula)
-  (v1 v2: val_vars gamma_valid i vt) 
+  (v1 v2: val_vars pd vt) 
   (Hval: valid_formula sigma f):
   (forall x, In x (form_fv f) -> v1 x = v2 x) ->
   formula_rep v1 f Hval = formula_rep v2 f Hval.
@@ -2459,7 +2474,7 @@ Qed.
   to a new variable without changing the truth value*)
 (*The proof is a straightforward application of [sub_f_correct]
   and [form_fv_agree], but the casts make it a bit tedious*)
-Lemma alpha_convert_quant (v: val_vars gamma_valid i vt) 
+Lemma alpha_convert_quant (v: val_vars pd vt) 
   (q: quant) (v1 v2: vsymbol) (Heq: snd v1 = snd v2) (f: formula)
   (Hval1: valid_formula sigma (Fquant q v1 f))
   (Hval2: valid_formula sigma (Fquant q v2 (sub_f v1 v2 f)))
@@ -2474,7 +2489,7 @@ Proof.
     split; intros Hall d.
     + inversion Hval1; subst.
       rewrite sub_f_correct with(Heq:=Heq)(Hval1:=H4); auto.
-      rewrite (form_fv_agree _ _ (substi vt v v1 (dom_cast (dom_aux gamma_valid i) (f_equal (val vt) (eq_sym Heq))
+      rewrite (form_fv_agree _ _ (substi vt v v1 (dom_cast (dom_aux pd) (f_equal (val vt) (eq_sym Heq))
       (substi vt v v2 d v2)))).
       2: {
         intros x Hinx. unfold substi. destruct (vsymbol_eq_dec x v2); auto.
@@ -2522,7 +2537,7 @@ Proof.
       rewrite sub_f_correct with (Heq:= (eq_sym (eq_trans (eq_sym Heq) Heqty))) 
         (Hval1:= (valid_quant_inj (valid_formula_eq eq_refl Hval1))); auto.
       rewrite (form_fv_agree _ _ (substi vt v v1
-      (dom_cast (dom_aux gamma_valid i)
+      (dom_cast (dom_aux pd)
          (f_equal (val vt) (eq_trans (eq_sym Heq) Heqty)) d))); auto.
       intros x Hinx.
       unfold substi.
@@ -2537,6 +2552,176 @@ Proof.
         subst; contradiction.
 Qed.
 
+Definition sublist {A: Type} (l: list A) (lo hi: nat) : list A.
+Admitted.
+
+(*Split a list into pieces of the appropriate lengths if we can*)
+Fixpoint split_lens {A: Type} (l: list A) (lens: list nat) :
+  list (list A) :=
+  match lens with
+  | len :: tl => sublist l 0 len :: 
+    split_lens (sublist l (len + 1) (length l)) tl
+  | nil => nil
+  end.
+
+(*If we know that the bound variable names are unique and do
+  not conflict with the free variable names, we can prove the
+  correctness of many transformations. We define such a notion
+  and provide a function (not necessarily the most efficient one)
+  to alpha-convert our term/formula into this form.*)
+(*TODO: make names consistent*)
+Definition term_wf (t: term) : Prop :=
+  NoDup (bnd_t t) /\ forall x, ~ (In x (term_fv t) /\ In x (bnd_t t)).
+Definition fmla_wf (f: formula) : Prop :=
+  NoDup (bnd_f f) /\ forall x, ~ (In x (form_fv f) /\ In x (bnd_f f)).
+
+(*Easier to have separate function for pattern*)
+(*Hmm, need to think a bit more - how should patterns work?
+  *)
+
+(*TODO: want bound variables for patterns because we care about
+  lengths*)
+
+(*Alpha substitute for patterns only in the given term/formula*)
+Fixpoint alpha_p_aux {A: Type} (sub: vsymbol -> vsymbol -> A -> A) 
+  (p: pattern) (x: A) (l: list string) : (pattern * A) :=
+  match p with
+  | Pvar v => 
+    match l with
+    | nil => (p, x)
+    | str :: tl =>
+      let v' := (str, snd v) in
+      (Pvar v', sub v v' x)
+    end
+  | Pwild => (p, x)
+  | Por p1 p2 =>
+    (*NOTE: must have same free vars*)
+    let (p1', x1) := alpha_p_aux sub p1 x l in
+    let (p2', x2) := alpha_p_aux sub p2 x l in
+    (Por p1 p2, x2)
+  | Pbind p1 v =>
+    match l with
+    |nil => (p, x)
+    | str :: tl =>
+      let v' := (str, snd v) in
+      let (p2, x1) := (alpha_p_aux sub p1 x tl) in
+      (p2, sub v v' x1)
+    end
+  | Pconstr f tys pats =>
+    (*Split list into lists of appropriate length*)
+    (*Split up the list into pieces of appropriate lengths 
+      (size (bnd_t tm))*)
+      let lens := map (fun tm => length (bnd_p tm)) pats in
+      let l_split := split_lens l lens in
+      let (ps', xnew) := ((fix alpha_ps_aux (l1: list pattern) (l2: list (list string)) (y: A) :
+        (list pattern * A) :=
+        match l1, l2 with
+        | (ph :: pt), (s1 :: st) =>
+            let (pnew, y1) := alpha_p_aux sub ph y s1 in
+            let (prest, y2) := alpha_ps_aux pt st y1 in
+            (pnew :: prest, y2)
+        | _, _ =>
+          (nil, y)
+        end) pats l_split x) in
+      (Pconstr f tys ps', xnew)
+    end.
+(*Proving this correct will not be too fun, but let's see*)
+(*
+Print term.
+Print bnd_t.
+Print sub_t.
+(*TOOD: might not be able to use map, see*)
+Fixpoint alpha_t_aux (t: term) (l: list string) {struct t} : term :=
+  (*We only care about the bound variable and inductive cases*)
+  match t with
+  | Tlet t1 x t2 => 
+    match l with
+    | str :: _ => Tlet t1 (str, snd x) (sub_t x (str, snd x) t2)
+    | _ => t
+    end
+  | Tfun fs tys tms =>
+    (*Split up the list into pieces of appropriate lengths 
+      (size (bnd_t tm))*)
+    let lens := map (fun tm => length (bnd_t tm)) tms in
+    let l_split := split_lens l lens in
+    Tfun fs tys (map (fun (t: term * list string) =>
+      let (tm, l') := t in alpha_t_aux tm l') (combine tms l_split))
+  | Tif f t1 t2 =>
+    let f_sz := length (bnd_f f) in
+    let t1_sz := length (bnd_t t1) in
+    Tif (alpha_f_aux f (sublist l 0 f_sz)) 
+      (alpha_t_aux t1 (sublist l (f_sz + 1) (f_sz + 1 + t1_sz)))
+      (alpha_t_aux t2 (sublist l (f_sz + 1 + t1_sz + 1) (length l)))
+  | Tmatch t1 ty ps =>
+    (*First do the pattern substitutions, then do the terms
+      recursively*)
+    let lens := map (fun x => length (bnd_p (fst x)) + 
+      length (bnd_t (snd x))) ps in
+    let l_split := split_lens l lens in
+    let t1_sz := length (bnd_t t1) in
+    Tmatch (alpha_t_aux t1 (sublist l 0 t1_sz)) ty
+      (map (fun (t: (pattern * term) * list string) => let (x, strs):= t in
+        let p_sz := length (bnd_p (fst x)) in
+        let l1 := sublist strs 0 p_sz in
+        let l2 := sublist strs p_sz (length strs) in
+        let (p1, y) := alpha_p_aux sub_t (fst x) (snd x) l1 in
+        (p1, alpha_t_aux y l2)
+        ) (combine ps l_split))
+  | Teps f v =>
+    match l with
+    | nil => t
+    | str :: tl =>
+      let v' := (str, snd v) in
+      Teps (sub_f v v' (alpha_f_aux f tl)) v'
+    end
+  | _ => t (*no other bound variables/recursive cases*)
+  end
+with alpha_f_aux (f: formula) (l: list string) {struct f} : formula :=
+  match f with
+  | Fpred ps tys tms =>
+    (*Split up the list into pieces of appropriate lengths 
+      (size (bnd_t tm))*)
+    let lens := map (fun tm => length (bnd_t tm)) tms in
+    let l_split := split_lens l lens in
+    Fpred ps tys (map (fun (t: term * list string) =>
+      let (tm, l') := t in alpha_t_aux tm l') (combine tms l_split))
+  | _ => f
+  end.
+
+    (fix alpha_ts_aux (l: list (pattern * term)) :
+      list (pattern * term)
+    let ps_p
+
+    (*harder*)
+    
+    Tmatch (alpha_t_aux t1 (sublist l 0 t1_sz)) ty
+      (fun (p: pattern * term) =>
+
+
+
+      
+      )
+
+
+
+
+    Tfun fs tys 
+  | Tconst _ => t
+  | Tvar v => t
+
+Lemma alpha_t_aux_correct (t: term) (l: list vsymbol),
+  NoDup l ->
+  (forall x, In x l -> ~ In x (map fst (term_fv t))) ->
+  length l = length (bnd_t t) ->
+  term_interp (alpha_t_aux t l) Hty =
+  term_interp t Hty /\
+  term_wf (alpha_t_aux t l).
+
+
+(*Let's try*)
+Definition 
+*)
+End Alpha.
 End Denot.
 
 (*
